(naming) ghost_simplified_model to casemate_model

src/casemate-check-rocq/src/menhir_parser.mly
@@ -24,7 +24,7 @@
 
 %start trans
 
-%type <ghost_simplified_model_transition> trans
+%type <casemate_model_step> trans
 
 %%
 
